\begin{itemize}
    \item[a)] 
    \begin{align*}
        \mathbb{E}\{X\} &=  
        \int_{-\infty}^{+\infty} x \cdot f_{X}(x) dx = 
        \int_{0}^{+\infty} x \cdot \lambda \cdot e^{-\lambda \cdot x} dx \\
        &= 
        \left[ -x \cdot e^{-\lambda \cdot x} \right]_{0}^{+\infty} \int_{0}^{+\infty} \cdot e^{-\lambda \cdot x} dx =
        0 + \left[ -\frac{1}{\lambda} \cdot e^{-\lambda \cdot x} \right]_{0}^{+\infty} = \frac{1}{\lambda}
    \end{align*}
    \item[b)]
        \begin{align*}
        \mathbb{H}(X) &=  
            -\int_{-\infty}^{+\infty} f_{X}(x) \cdot \text{ln} \left( f_{X}(x) \right) dx = 
            -\int_{0}^{+\infty} x \cdot \lambda \cdot e^{-\lambda \cdot x} \cdot \text{ln} \left( x \cdot \lambda \cdot e^{-\lambda \cdot x} \right) dx 
            \\ &=
            -\text{ln}(\lambda) \underbrace{\int_{0}^{+\infty} \lambda \cdot e^{-\lambda \cdot x} dx }_{=1} 
            + \lambda \underbrace{ \int_{0}^{+\infty} x \cdot \lambda \cdot e^{-\lambda \cdot x} dx }_{1/\lambda} = 1 - \text{ln}(\lambda)
    \end{align*}
    \item[c)]
    \begin{align*}
        \mathbb{D}(X\| Y) &=  
            \int_{-\infty}^{+\infty} f_{X}(x) \cdot \text{ln} \left( \frac{f_{X}(x)}{f_{Y}(x)} \right) dx 
            \\&= 
            \underbrace{\int_{-\infty}^{+\infty} f_{X}(x) \cdot \text{ln} \left( f_{X}(x) \right) dx }_{=-H(X)}
            - \int_{-\infty}^{+\infty} f_{X}(x) \cdot \text{ln} \left( f_{Y}(x) \right) dx
            \\ &=
            -(1 -\text{ln}(\lambda) ) - \int_{-\infty}^{+\infty} x \cdot \lambda \cdot e^{-\lambda \cdot x} \cdot \text{ln} \left( x \cdot \xi \cdot e^{-\xi \cdot x} \right) dx
            \\ &=
             \text{ln}(\lambda) -1 - \text{ln}(\xi) \underbrace{\int_{-\infty}^{+\infty} \lambda \cdot e^{-\lambda \cdot x} dx }_{=1} + \xi \underbrace{\int_{-\infty}^{+\infty} x \cdot \lambda \cdot e^{-\lambda \cdot x} dx }_{=1/\lambda}
            \\ &=
            -1 + \text{ln}(\lambda) - \text{ln}(\xi) + \frac{\xi}{\lambda} = \frac{\xi}{\lambda} - \text{ln}(\frac{\xi}{\lambda}) - 1
     \end{align*}
    
    Since $\mathbb{D}(X\| Y) \geq 0$ we get $\frac{\xi}{\lambda} - \text{ln}\left(\frac{\xi}{\lambda}\right) - 1 \geq 0$. Then, by defining $\alpha \in \mathbb{R}^{+}$ as $\alpha =  \frac{\xi}{\lambda}$ we get
    $$
    \alpha - \text{ln}(\alpha) - 1 \geq 0 \qquad \Rightarrow \qquad \alpha - 1 \geq \text{ln}(\alpha) \, .
    $$
    \item[d)]
    \begin{align*}
        H(N) &= -\sum_{n = -\infty}^{+\infty} f_{N}(n) \text{log}_2 \left( f_{N}(n) \right) \\
        &= -\sum_{n = 1}^{+\infty} \left( \frac{1}{2} \right)^{n} \text{log}_2 \left( \left( \frac{1}{2} \right)^{n} \right)
        = \sum_{n = 1}^{+\infty} n \cdot \left( \frac{1}{2} \right)^{n} \\
        &= \frac{\frac{1}{2}}{\left(1 - \frac{1}{2}\right)^2} = 2
    \end{align*}
    \item[e)] $N_1$ and $N_2$ follow the same distribution as $N$, and they are also independent random variables.
    \item[f)] $H(S) = H(N_1 + N_2) \leq H(N_1, N_2) = H(N_1) + H(N_2) = 2 H(N)$ .
    
\end{itemize}